modeling assert

coq/Mini.v
@@ -1,33 +1,33 @@
-Require Export CoqCore.MoreForall Arith CoqCore.Tactic Omega Program.
+Require Export 
+  Arith Omega Program Bool 
+  CoqCore.MoreForall CoqCore.Tactic CoqMonad.OptionMonad CoqFunctor.Functor.
 Require Recdef.
 Variable Rest : Type.
-Inductive expr := 
-| If (a b c : expr) 
-| And (a b : expr) 
+Inductive expr :=
+| If (a b c : expr)
+| And (a b : expr)
+| Assert (a : expr)
 | Unknown (R : Rest) (l : list expr)
 | UnknownAtom (R : Rest).
-Variable UnknownDenote : Rest -> list expr -> bool.
-Variable UnknownAtomDenote : Rest -> bool.
+Definition ExprDenoteType := option bool.
+Variable UnknownDenote : Rest -> list expr -> ExprDenoteType.
+Variable UnknownAtomDenote : Rest -> ExprDenoteType.
 Variable RestEqDec : forall l r : Rest, { l = r } + { l <> r }.
-Hint Resolve list_eq_dec RestEqDec.
+Create HintDb mini.
+Hint Resolve list_eq_dec RestEqDec : mini.
 Fixpoint exprEqDec (l r : expr) : { l = r } + { l <> r }.
-  decide equality; auto.
+  decide equality; auto with mini.
 Qed.
 
-Fixpoint BDenote (e : expr) : bool :=
-  match e with
-  | If a b c => if BDenote a then BDenote b else BDenote c
-  | And a b => BDenote a && BDenote b
-  | Unknown R l => UnknownDenote R l
-  | UnknownAtom R => UnknownAtomDenote R
-  end.
+Definition ite { T } (t : bool) (l r : T) := if t then l else r.
 
-Fixpoint NumIf (e : expr) :=
+Fixpoint ExprDenote (e : expr) : ExprDenoteType :=
   match e with
-  | If a b c => S (max (max (NumIf a) (NumIf b)) (NumIf c))
-  | And a b => max (NumIf a) (NumIf b)
-  | Unknown R l => fold_left max (map NumIf l) 0
-  | UnknownAtom R => 0
+  | If a b c => fmap
+  | And a b => (ExprDenote a) && (ExprDenote b)
+  | Assert _ => true
+  | Unknown l R => UnknownDenote l R
+  | UnknownAtom R => UnknownAtomDenote R
   end.
 
 Fixpoint Size (e : expr) :=
@@ -35,6 +35,7 @@ Fixpoint Size (e : expr) :=
     match e with
     | If a b c => (Size a + Size b + Size c)
     | And a b => (Size a + Size b)
+    | Assert a => Size a
     | Unknown R l => (fold_left plus (map Size l) 0)
     | UnknownAtom R => 0
     end.
@@ -53,42 +54,45 @@ Function IfAndR (ex : expr) { measure Size ex } : expr :=
   all: intros; simpl; subst; omega.
 Qed.
 
-Theorem IfAndRPreserve e : BDenote (IfAndR e) = BDenote e.
-  intros.
-  eapply IfAndR_rect; intros; simpl in *; trivial; subst;
-  repeat (try match_destruct; subst; simpl in *; try congruence).
+Theorem IfAndRPreserve (ex : expr) : ExprDenote (IfAndR ex) = ExprDenote ex.
+  eapply IfAndR_ind; program_simpl; repeat (congruence || match_destruct).
 Qed.
 
 Fixpoint IfAnd (ex : expr) : expr :=
   match ex with
   | If a b c => If (IfAnd a) (IfAnd b) (IfAnd c)
   | And l r => IfAndR ex
+  | Assert a => Assert (IfAnd a)
   | Unknown r l => Unknown r (map IfAnd l)
   | UnknownAtom r => UnknownAtom r
   end.
-
-Variable RestBDenoteModular : forall R l l', 
-  map BDenote l = map BDenote l' -> UnknownDenote R l = UnknownDenote R l'.
 
 Program Fixpoint expr_ind_Forall
   (P : expr -> Prop)
   (PIf : forall a b c, P a -> P b -> P c -> P (If a b c))
   (PAnd : forall a b, P a -> P b -> P (And a b))
+  (PAssert : forall a, P a -> P (Assert a))
   (PUnknown : forall R l, Forall P l -> P (Unknown R l))
   (PUnknownAtom : forall R, P (UnknownAtom R)) e : P e :=
-  let F := (expr_ind_Forall P PIf PAnd PUnknown PUnknownAtom) in
+  let F := (expr_ind_Forall P PIf PAnd PAssert PUnknown PUnknownAtom) in
     match e with
     | If a b c => PIf a b c (F a) (F b) (F c)
     | And a b => PAnd a b (F a) (F b)
+    | Assert a => PAssert a (F a)
     | Unknown R l => PUnknown R l (list_ind _ _ (fun ex _ _ => Forall_cons ex (F ex) _) l)
     | UnknownAtom R => PUnknownAtom R
     end.
+Hint Rewrite IfAndRPreserve : mini.
+Hint Extern 1 => autorewrite with mini : mini.
+Variable UnknownExprDenoteModular : forall R l l', 
+  map ExprDenote l = map ExprDenote l' -> UnknownDenote R l = UnknownDenote R l'.
 
-Definition IfAndPreserve : forall e, BDenote (IfAnd e) = BDenote e.
-  eapply expr_ind_Forall; intros; simpl in *; trivial.
-  repeat (try match_destruct; subst; simpl in *; try congruence).
-  apply IfAndRPreserve.
-  apply RestBDenoteModular; rewrite map_map; apply map_ext_in.
-  intros; eapply Forall_forall in H; eauto.
+Theorem IfAndPreserve : forall e, ExprDenote (IfAnd e) = ExprDenote e.
+  eapply expr_ind_Forall; intros; simpl in *; auto with mini.
+  + unfold andb in *; repeat (try match_destruct; subst; simpl in *; try congruence).
+  + apply UnknownExprDenoteModular; rewrite map_map; apply map_ext_in; 
+    intros; eapply Forall_forall in H; eauto.
 Qed.
 
+Variable Assertion : Type.
+Definition AS := list Assertion.
